tests/lean/Avl/Tree.lean
@@ -1,5 +1,6 @@
 import Avl.Funs
 import Avl.Types
+-- TODO: merge into Spec.lean
 
 namespace avl
 
@@ -16,7 +17,18 @@ def Node.compute_height: Node T -> Nat
 @[simp]
 def Child.compute_height: Child T -> Nat
 | none => 0
-| some n => 1 + Node.compute_height n
+| some n => Node.compute_height n
+end
+
+mutual
+@[simp]
+def Node.size: Node T -> Nat
+| Node.mk y left right _ => 1 + Child.size left + Child.size right
+
+@[simp]
+def Child.size: Child T -> Nat
+| none => 0
+| some n => 1 + Node.size n
 end
 
 def Tree.nil: Tree T := { root := none }
@@ -29,16 +41,17 @@ instance [Inhabited T]: Inhabited (Node T) where
   default := ⟨ Inhabited.default, none, none, 0#usize ⟩
 
 mutual
-@[simp] def Child.v (tree: Child T) : Set T :=
+@[simp, reducible] def Child.v (tree: Child T) : Set T :=
   match tree with
   | none => ∅
   | some node => node.v
 
-@[simp] def Node.v (node : Node T) : Set T :=
+@[simp, reducible] def Node.v (node : Node T) : Set T :=
   match node with
   | .mk x left right _ => {x} ∪ Child.v left ∪ Child.v right
 end
 
+@[reducible]
 def Tree.v (t: Tree T): Set T := Child.v t.root
 
 end avl
