tests/lean/Avl.lean
@@ -1,5 +1,4 @@
 import Avl.Insert
 import Avl.Find
-import Avl.Order
 import Avl.Height
 import Avl.Rotate
