tests/lean/Avl/OrderSpec.lean
@@ -121,4 +121,37 @@ theorem gtOfRustOrder
   rewrite [oppositeRustOrder]
   simp [Hcmp]
 
+-- TODO: move to standard library
+@[simp]
+theorem compare_eq_lt_iff [LinOrd : LinearOrder T] (x y : T) :
+  compare x y = Ordering.lt ↔ x < y := by
+  simp_all [LinOrd.compare_eq_compareOfLessAndEq, compareOfLessAndEq]
+  split <;> simp_all
+
+-- TODO: move to standard library
+@[simp]
+theorem compare_eq_equal_iff [LinOrd : LinearOrder T] (x y : T) :
+  compare x y = Ordering.eq ↔ x = y := by
+  simp_all [LinOrd.compare_eq_compareOfLessAndEq, compareOfLessAndEq]
+  split <;> simp_all
+  rw [eq_iff_le_not_lt]
+  tauto
+
+-- TODO: move to standard library
+@[simp]
+theorem compare_eq_gt_iff [LinOrd : LinearOrder T] (x y : T) :
+  compare x y = Ordering.gt ↔ y < x := by
+  simp_all [LinOrd.compare_eq_compareOfLessAndEq, compareOfLessAndEq]
+  split <;> simp_all
+  . rw [lt_iff_le_not_le] at *; tauto
+  . constructor
+    . intro Hneq
+      apply lt_of_le_of_ne <;> tauto
+    . intro Hlt
+      rw [eq_iff_le_not_lt]
+      simp
+      intro Hle
+      have := le_antisymm Hle
+      simp_all
+
 end avl
